P1.fst
@@ -1,0 +1,356 @@
+module P1
+
+
+open FStar.Ghost
+
+open Steel.Memory
+open Steel.Effect.Atomic
+open Steel.Effect
+open Steel.Reference
+
+module Spec = Trees
+
+open NTreeC3
+/// The implementation of the Selectors.Tree interface.
+/// Predicates prefixed by (**) correspond to stateful lemmas for folding and unfolding the tree predicate
+
+#set-options "--fuel 1 --ifuel 1 --z3rlimit 50 --ide_id_info_off"
+
+let rec append_left #a (ptr: t a) (v: a)
+  : Steel (t a)
+  (linked_tree ptr)
+  (fun ptr' ->  linked_tree ptr')
+  (requires (fun h0 -> True))
+  (ensures (fun h0 ptr' h1 -> v_linked_tree ptr' h1 == Spec.append_left (v_linked_tree ptr h0) v))
+  =
+  if is_null_t ptr then (
+    (**) elim_linked_tree_leaf ptr;
+    let sr = malloc 1 in
+    let node = mk_node v ptr null_t sr in
+    let new_tree = malloc node in
+    (**) intro_linked_tree_leaf #a ();
+    (**) pack_tree new_tree ptr null_t sr;
+    new_tree
+    // return new_tree
+  ) else (
+    let h1 = get () in
+    (**) let node = NTreeC3.unpack_tree ptr in
+    let h2 = get () in
+
+    let ptr_t1 = hide (v_linked_tree ptr h1) in
+    let ptr_t2 = hide (Spec.Node
+      (get_data (sel ptr h2))
+      (v_linked_tree (get_left node) h2)
+      (v_linked_tree (get_right node) h2)
+      (sel (get_size node) h2)) in
+    assert (reveal ptr_t1 == reveal ptr_t2);
+    assert (fst (Spec.is_wds ptr_t1));
+    assert (fst (Spec.is_wds ptr_t2));
+    let ptr_s1 = hide (Spec.csize (reveal ptr_t1)) in
+    let ptr_s2 = hide (Spec.csize (reveal ptr_t2)) in
+    assert (reveal ptr_s1 == reveal ptr_s2);
+    Spec.check (reveal ptr_t1);
+    assert (reveal ptr_s1 == Spec.size_of_tree (reveal ptr_t1));
+
+    (**) let new_left = append_left (get_left node) v in
+    let h3 = get () in
+    let old_left_t = hide (v_linked_tree (get_left node) h2) in
+    let new_left_t = hide (v_linked_tree new_left h3) in
+    let old_left_s = hide (Spec.size_of_tree (reveal old_left_t)) in
+    let new_left_s = hide (Spec.size_of_tree (reveal new_left_t)) in
+    let old_right_t = hide (v_linked_tree (get_right node) h2) in
+    let new_right_t = hide (v_linked_tree (get_right node) h3) in
+    let old_right_s = hide (Spec.size_of_tree (reveal old_right_t)) in
+    let new_right_s = hide (Spec.size_of_tree (reveal new_right_t)) in
+    assert (fst (Spec.is_wds (reveal ptr_t2)));
+    assert (reveal ptr_s2 == reveal old_left_s + reveal old_right_s + 1);
+
+    assert (fst (Spec.is_wds (reveal old_left_t)));
+    assert (fst (Spec.is_wds (reveal new_left_t)));
+    assert (old_right_t == new_right_t);
+    assert (fst (Spec.is_wds old_right_t));
+    Spec.append_left_aux_size (reveal old_left_t) v;
+    assert (reveal new_left_s == reveal old_left_s + 1);
+    assert (reveal old_right_s == reveal new_right_s);
+
+    // TODO : incr (get_size node);
+    let old_size = read (get_size node) in
+    (***) write (get_size node) (old_size + 1);
+    let h4 = get () in
+    assert (sel (get_size node) h4 == sel (get_size node) h3 + 1);
+    assert (sel (get_size node) h4 == new_left_s + new_right_s + 1);
+
+    let new_node = mk_node (get_data node) new_left (get_right node) (get_size node) in
+    assert (get_size new_node == get_size node);
+    (***) write ptr new_node;
+
+    (**) pack_tree ptr new_left (get_right node) (get_size node);
+    return ptr
+  )
+
+// Alternative possible dans le corps de la fonction suivante
+//free old_sr;
+//let new_sr = malloc (old_size + 1) in
+
+(*)
+let rec append_left #a ptr v =
+  if is_null_t ptr then (
+    (**) elim_linked_tree_leaf ptr;
+    let node = mk_node v ptr null_t in
+    let new_tree = malloc node in
+    (**) intro_linked_tree_leaf #a ();
+    (**) pack_tree new_tree ptr null_t;
+    new_tree
+  ) else (
+    (**) let node = unpack_tree ptr in
+    let new_left = append_left (get_left node) v in
+    let new_node = mk_node (get_data node) new_left (get_right node) in
+    write ptr new_node;
+    (**) pack_tree ptr new_left (get_right node);
+    ptr
+  )
+
+let rec append_right #a ptr v =
+  if is_null_t ptr then (
+    (**) elim_linked_tree_leaf ptr;
+    let node = mk_node v null_t ptr in
+    let new_tree = malloc node in
+    (**) intro_linked_tree_leaf #a ();
+    (**) pack_tree new_tree null_t ptr;
+    new_tree
+  ) else (
+    (**) let node = unpack_tree ptr in
+    let new_right = append_right (get_right node) v in
+    let new_node = mk_node (get_data node) (get_left node) new_right in
+    write ptr new_node;
+    (**) pack_tree ptr (get_left node) new_right;
+    ptr
+  )
+
+let rec height #a ptr =
+   if is_null_t ptr then (
+     (**) elim_linked_tree_leaf ptr;
+     0
+   ) else (
+     (**) let node = unpack_tree ptr in
+     let hleft = height (get_left node) in
+     let hright = height (get_right node) in
+     (**) pack_tree ptr (get_left node) (get_right node);
+     if hleft > hright then (
+       hleft + 1
+     ) else ( hright + 1 )
+   )
+
+let rec member ptr v =
+  if is_null_t ptr then (
+    (**) elim_linked_tree_leaf ptr;
+    false
+  ) else (
+    (**) let node = unpack_tree ptr in
+    if v = get_data node then (
+      (**) pack_tree ptr (get_left node) (get_right node);
+      true
+    ) else (
+      let mleft = member (get_left node) v in
+      let mright = member (get_right node) v in
+      (**) pack_tree ptr (get_left node) (get_right node);
+      mleft || mright
+    )
+  )
+
+#push-options "--ifuel 1 --fuel 2"
+let rotate_left #a ptr =
+  (**) node_is_not_null ptr;
+  (**) let x_node = unpack_tree ptr in
+  let x = get_data x_node in
+  (**) node_is_not_null (get_right x_node);
+  (**) let z_node = unpack_tree (get_right x_node) in
+  let z = get_data z_node in
+  let new_subnode = mk_node x (get_left x_node) (get_left z_node) in
+  let new_node = mk_node z ptr (get_right z_node) in
+  write (get_right x_node) new_node;
+  write ptr new_subnode;
+  (**) pack_tree ptr (get_left x_node) (get_left z_node);
+  (**) pack_tree (get_right x_node) ptr (get_right z_node);
+  (get_right x_node)
+
+let rotate_right #a ptr =
+  (**) node_is_not_null ptr;
+  (**) let x_node = unpack_tree ptr in
+  let x = get_data x_node in
+  (**) node_is_not_null (get_left x_node);
+  let z_node = unpack_tree (get_left x_node) in
+  let z = get_data z_node in
+  let new_subnode = mk_node x (get_right z_node) (get_right x_node) in
+  let new_node = mk_node z (get_left z_node) ptr in
+  write (get_left x_node) new_node;
+  write ptr new_subnode;
+  (**) pack_tree ptr (get_right z_node) (get_right x_node);
+  (**) pack_tree (get_left x_node) (get_left z_node) ptr;
+  (get_left x_node)
+
+
+let rotate_right_left #a ptr =
+  (**) node_is_not_null ptr;
+  // original root node
+  (**) let x_node = unpack_tree ptr in
+  let x = get_data x_node in
+  (**) node_is_not_null (get_right x_node);
+  // original right node
+  // z = get_right x_node
+  (**) let z_node = unpack_tree (get_right x_node) in
+  let z = get_data z_node in
+  (**) node_is_not_null (get_left z_node);
+  // original left (right node)
+  // y = get_left (z_node)
+  (**) let y_node = unpack_tree (get_left z_node) in
+  let y = get_data y_node in
+  let new_x = mk_node x (get_left x_node) (get_left y_node) in
+  let new_z = mk_node z (get_right y_node) (get_right z_node) in
+  let new_y = mk_node y ptr (get_right x_node) in
+
+  write ptr new_x;
+  write (get_right x_node) new_z;
+  write (get_left z_node) new_y;
+
+  (**) pack_tree ptr (get_left x_node) (get_left y_node);
+  (**) pack_tree (get_right x_node) (get_right y_node) (get_right z_node);
+  (**) pack_tree (get_left z_node) ptr (get_right x_node);
+
+  (get_left z_node)
+
+
+let rotate_left_right #a ptr =
+  (**) node_is_not_null ptr;
+  // original root node
+  (**) let x_node = unpack_tree ptr in
+  let x = get_data x_node in
+
+  (**) node_is_not_null (get_left x_node);
+
+  // original left node
+  // z = get_left x_node
+  (**) let z_node = unpack_tree (get_left x_node) in
+  let z = get_data z_node in
+
+  (**) node_is_not_null (get_right z_node);
+
+  // original right (left node)
+  // y = get_right (z_node)
+  (**) let y_node = unpack_tree (get_right z_node) in
+  let y = get_data y_node in
+
+  let new_z = mk_node z (get_left z_node) (get_left y_node) in
+  let new_x = mk_node x (get_right y_node) (get_right x_node) in
+  let new_y = mk_node y (get_left x_node) ptr in
+
+  write (get_left x_node) new_z;
+  write ptr new_x;
+  write (get_right z_node) new_y;
+
+  (**) pack_tree (get_left x_node) (get_left z_node) (get_left y_node);
+  (**) pack_tree ptr (get_right y_node) (get_right x_node);
+  (**) pack_tree (get_right z_node) (get_left x_node) ptr;
+
+  (get_right z_node)
+
+let rec is_balanced #a ptr =
+  if is_null_t ptr then (
+    (**) elim_linked_tree_leaf ptr;
+    true
+  ) else (
+
+  (**) let node = unpack_tree ptr in
+  let lh = height (get_left node) in
+  let rh = height (get_right node) in
+
+  let lbal = is_balanced(get_left node) in
+  let rbal = is_balanced(get_right node) in
+
+  (**) pack_tree ptr (get_left node) (get_right node);
+  (lbal && rbal) && ((rh - lh) >= -1 && (rh - lh) <= 1))
+
+#push-options "--ifuel 2"
+let rebalance_avl #a cmp ptr =
+  if is_balanced ptr then (
+    return ptr
+  ) else (
+
+    (**) node_is_not_null ptr;
+    (**) let node = unpack_tree ptr in
+
+    let lh = height (get_left node) in
+    let rh = height (get_right node) in
+
+    if (lh - rh) > 1 then (
+
+      (**) node_is_not_null (get_left node);
+      (**) let l_node = unpack_tree (get_left node) in
+
+      let llh = height (get_left l_node) in
+      let lrh = height (get_right l_node) in
+
+      (**) pack_tree (get_left node) (get_left l_node) (get_right l_node);
+      (**) pack_tree ptr (get_left node) (get_right node);
+
+      if lrh > llh then (
+        rotate_left_right ptr
+
+      ) else (
+        rotate_right ptr
+      )
+
+    ) else (
+
+      if (lh - rh) < - 1 then (
+
+        (**) node_is_not_null (get_right node);
+        (**) let r_node = unpack_tree (get_right node) in
+
+        let rlh = height (get_left r_node) in
+        let rrh = height (get_right r_node) in
+
+        (**) pack_tree (get_right node) (get_left r_node) (get_right r_node);
+        (**) pack_tree ptr (get_left node) (get_right node);
+
+        if rlh > rrh then (
+          rotate_right_left ptr
+        ) else (
+          rotate_left ptr
+        )
+
+      ) else (
+        (**) pack_tree ptr (get_left node) (get_right node);
+        ptr
+      )
+    )
+  )
+#pop-options
+
+let rec insert_avl #a cmp ptr v =
+  if is_null_t ptr then (
+    (**) elim_linked_tree_leaf ptr;
+    let node = mk_node v ptr null_t in
+    let new_tree = malloc node in
+    (**) intro_linked_tree_leaf #a ();
+    (**) pack_tree new_tree ptr null_t;
+    new_tree
+  ) else (
+    (**) let node = unpack_tree ptr in
+    if cmp (get_data node) v >= 0 then (
+      let new_left = insert_avl cmp (get_left node) v in
+      let new_node = mk_node (get_data node) new_left (get_right node) in
+      write ptr new_node;
+      (**) pack_tree ptr new_left (get_right node);
+      rebalance_avl cmp ptr
+    )
+    else (
+      let new_right = insert_avl cmp (get_right node) v in
+      let new_node = mk_node (get_data node) (get_left node) new_right in
+      write ptr new_node;
+      (**) pack_tree ptr (get_left node) new_right;
+      rebalance_avl cmp ptr
+    )
+  )
+
+#pop-options
